Tests/DTLC/TypSpec.lean
@@ -1,0 +1,50 @@
+import «Lp2lc».Active.DTLC.Def
+
+namespace Tests.DTLC.Sanity
+open Lp2lc.Active.DTLC
+
+namespace Typ
+
+def false : TypAST :=
+  .primitive
+
+def idFn : TypAST :=
+  .depFn .primitive (fun _x => .primitive)
+
+def get1st : TypAST :=
+  .depFn .primitive (fun _x =>
+    .depFn .primitive (fun _y => .primitive))
+
+def apply1stOn2ndFn : TypAST :=
+  .depFn
+    (.depFn .primitive (fun _x => .primitive))
+    (fun _f =>
+      .depFn .primitive (fun _x => .primitive))
+
+end Typ
+
+-- namespace Typing
+
+-- example : TrmClosed.typing Trm.false 2 Typ.false := by
+--   simp [TrmClosed.typing, Trm.false, Typ.false]
+
+-- example : TrmClosed.typing Trm.true 2 Typ.true := by
+--   simp [TrmClosed.typing, Trm.true, Typ.true]
+
+-- example : TrmClosed.typing Trm.idFn 3 Typ.idFn := by
+--   simp [TrmClosed.typing, Trm.idFn, Typ.idFn]
+
+-- example : TrmClosed.typing Trm.get1st 4 Typ.get1st := by
+--   simp [TrmClosed.typing, Trm.get1st, Typ.get1st]
+
+-- example : TrmClosed.typing Trm.get2nd 4 Typ.get2nd := by
+--   simp [TrmClosed.typing, Trm.get2nd, Typ.get2nd]
+
+-- example : ¬ TrmClosed.typing Trm.apply1stOn2ndFnOnTuple 6 Typ.apply1stOn2ndFnOnTuple := by
+--   simp [TrmClosed.typing, Trm.apply1stOn2ndFnOnTuple, Trm.apply1stOn2ndFn, Trm.idFn,
+--     Trm.false,
+--     Typ.apply1stOn2ndFnOnTuple]
+
+-- end Typing
+
+end Sanity
