Tests/DTLC/ValSpec.lean
@@ -1,0 +1,13 @@
+import «Lp2lc».Active.DTLC.Def
+
+namespace Tests.DTLC.Sanity
+open Lp2lc.Active.DTLC
+
+namespace Val
+
+def idFn : ValAST :=
+  .fn (body := fun x => .ref x)
+
+end Val
+
+end Sanity
