Tests/DTLC/package.lean
@@ -1,0 +1,3 @@
+import Tests.DTLC.ValSpec
+import Tests.DTLC.TrmSpec
+import Tests.DTLC.TypSpec
