Tests/package.lean
@@ -1,4 +1,4 @@
 
 import Tests.EquivIsoDemo
 import Tests.DOT.Sanity
-import Tests.DTLC.Sanity
+import Tests.DTLC.package
